template-coq/theories/Erasure/WcbvEval.v
@@ -2,6 +2,7 @@
 
 From Coq Require Import Bool String List Program BinPos Compare_dec Omega.
 From Template Require Import Template utils Ast univ Induction LiftSubst UnivSubst Typing.
+From Template.Erasure Require Import Ast.
 From Template Require AstUtils.
 Require Import String.
 Local Open Scope string_scope.
@@ -31,9 +32,10 @@ Section Wcbv.
   Inductive eval : term -> term -> Prop :=
   (** Reductions *)
   (** Beta *)
-  | eval_beta f na t b a l res :
+  | eval_beta f na t b a a' l res :
       eval f (tLambda na t b) ->
-      eval (mkApps (subst0 a b) l) res ->
+      eval a a' ->
+      eval (mkApps (subst0 a' b) l) res ->
       eval (tApp f (a :: l)) res
 
   (** Let *)
@@ -81,17 +83,26 @@ Section Wcbv.
   (* TODO CoFix *)
   | eval_abs na M N : eval (tLambda na M N) (tLambda na M N)
 
-  | eval_app_constr f i k u l l' :
+  | eval_prod na b t b' t' :
+      eval b b' -> eval t t' -> eval (tProd na b t) (tProd na b' t')
+
+  | eval_ind_ i u : eval (tInd i u) (tInd i u)
+
+  | eval_app_ind t i u l l' : l <> nil ->
+      eval t (tInd i u) ->
+      Forall2 eval l l' ->
+      eval (tApp t l) (tApp (tInd i u) l')
+
+  | eval_constr i k u :
+      eval (tConstruct i k u) (tConstruct i k u)
+
+  | eval_app_constr f i k u l l' : l <> nil ->
       eval f (tConstruct i k u) ->
       Forall2 eval l l' ->
-      eval (mkApps f l) (mkApps (tConstruct i k u) l')
-
-  (* | prod_eval_l na na' M1 M2 N1 : eval M1 N1 -> eval (tProd na M1 M2) (tProd na' N1 M2) *)
-  (* | prod_eval_r na na' M2 N2 M1 : red1 Σ (Γ ,, vass na M1) M2 N2 -> *)
-  (*                                 eval (tProd na M1 M2) (tProd na' M1 N2) *)
+      eval (tApp f l) (tApp (tConstruct i k u) l')
 
   (* | evar ev l l' : evals l l' -> eval (tEvar ev l) (tEvar ev l') *)
-  | evar_value ev l : eval (tEvar ev l) (tEvar ev l) (* Lets say it is a value for now *)
+  | eval_evar ev l : eval (tEvar ev l) (tEvar ev l) (* Lets say it is a value for now *)
 
   | eval_cast M1 k M2 N1 : eval M1 N1 -> eval (tCast M1 k M2) N1.
 
@@ -99,60 +110,89 @@ Section Wcbv.
 
   Lemma eval_evals_ind :
     forall P : term -> term -> Prop,
-      (forall (f : term) (na : name) (t b a : term) (l : list term) (res : term),
+      (forall (f : term) (na : name) (t b a a' : term) (l : list term) (res : term),
           eval f (tLambda na t b) ->
           P f (tLambda na t b) ->
-          eval (mkApps (b {0 := a}) l) res -> P (mkApps (b {0 := a}) l) res -> P (tApp f (a :: l)) res) ->
+          eval a a' -> P a a' ->
+          eval (mkApps (b {0 := a'}) l) res -> P (mkApps (b {0 := a'}) l) res -> P (tApp f (a :: l)) res) ->
+
       (forall (na : name) (b0 b0' t b1 res : term),
           eval b0 b0' -> P b0 b0' -> eval (b1 {0 := b0'}) res -> P (b1 {0 := b0'}) res -> P (tLetIn na b0 t b1) res) ->
+
       (forall (i : nat) (isdecl : i < #|Γ|) (body res : term),
           decl_body (safe_nth Γ (exist (fun n : nat => n < #|Γ|) i isdecl)) = Some body ->
           eval ((lift0 (S i)) body) res -> P ((lift0 (S i)) body) res -> P (tRel i) res) ->
+
       (forall (i : nat) (isdecl : i < #|Γ|),
           decl_body (safe_nth Γ (exist (fun n : nat => n < #|Γ|) i isdecl)) = None -> P (tRel i) (tRel i)) ->
+
       (forall (ind : inductive) (pars : nat) (discr : term) (c : nat) (u : universe_instance)
               (args : list term) (p : term) (brs : list (nat * term)) (res : term),
           eval discr (mkApps (tConstruct ind c u) args) ->
           P discr (mkApps (tConstruct ind c u) args) ->
           eval (iota_red pars c args brs) res ->
           P (iota_red pars c args brs) res -> P (tCase (ind, pars) p discr brs) res) ->
+
       (forall (mfix : mfixpoint term) (idx : nat) (args args' : list term) (narg : nat) (fn res : term),
           unfold_fix mfix idx = Some (narg, fn) ->
           Forall2 eval args args' ->
           Forall2 P args args' ->
           is_constructor narg args' = true ->
           eval (mkApps fn args') res -> P (mkApps fn args') res -> P (mkApps (tFix mfix idx) args) res) ->
+
       (forall (c : ident) (decl : constant_body) (body : term),
           declared_constant Σ c decl ->
           forall (u : universe_instance) (res : term),
             cst_body decl = Some body ->
             eval (subst_instance_constr u body) res -> P (subst_instance_constr u body) res -> P (tConst c u) res) ->
+
       (forall (i : inductive) (pars arg : nat) (discr : term) (args : list term) (k : nat)
               (u : universe_instance) (res : term),
           eval discr (mkApps (tConstruct i k u) args) ->
           P discr (mkApps (tConstruct i k u) args) ->
           eval (nth (pars + arg) args tDummy) res ->
           P (nth (pars + arg) args tDummy) res -> P (tProj (i, pars, arg) discr) res) ->
+
       (forall (na : name) (M N : term), P (tLambda na M N) (tLambda na M N)) ->
+
+      (forall (na : name) (M M' N N' : term),
+          eval M M' -> eval N N' -> P M M' -> P N N' ->
+          P (tProd na M N) (tProd na M' N')) ->
+
+      (forall i u, P (tInd i u) (tInd i u)) ->
+
+      (forall (f8 : term) (i : inductive) (u : universe_instance) (l l' : list term),
+          l <> nil -> eval f8 (tInd i u) ->
+          P f8 (tInd i u) -> Forall2 eval l l' -> Forall2 P l l' -> P (tApp f8 l) (tApp (tInd i u) l')) ->
+
+      (forall i k u, P (tConstruct i k u) (tConstruct i k u)) ->
+
       (forall (f8 : term) (i : inductive) (k : nat) (u : universe_instance) (l l' : list term),
-          eval f8 (tConstruct i k u) ->
-          P f8 (tConstruct i k u) -> Forall2 eval l l' -> Forall2 P l l' -> P (mkApps f8 l) (mkApps (tConstruct i k u) l')) ->
+          l <> nil -> eval f8 (tConstruct i k u) ->
+          P f8 (tConstruct i k u) -> Forall2 eval l l' -> Forall2 P l l' -> P (tApp f8 l) (tApp (tConstruct i k u) l')) ->
+
       (forall (ev : nat) (l : list term), P (tEvar ev l) (tEvar ev l)) ->
+
       (forall (M1 : term) (k : cast_kind) (M2 N1 : term), eval M1 N1 -> P M1 N1 -> P (tCast M1 k M2) N1) ->
+
       forall t t0 : term, eval t t0 -> P t t0.
   Proof.
-    intros P Hbeta Hlet Hreldef Hrelvar Hcase Hfix Hconst Hproj Hlam Hcstr Hevar Hcast.
+    intros P Hbeta Hlet Hreldef Hrelvar Hcase Hfix Hconst Hproj Hlam Hprod Hind Hindapp Hcstr Hcstrapp Hevar Hcast.
     fix 3. destruct 1;
-             match goal with [ H : _ |- _ ] =>
+             try match goal with [ H : _ |- _ ] =>
                              match type of H with
                                forall t t0, eval t t0 -> _ => fail 1
                              | _ => eapply H
                              end end; eauto.
     clear H1 H2.
-    revert args args' H0. fix 3. destruct 1. constructor; auto.
-    constructor. now apply eval_evals_ind. now apply eval_evals_ind0.
-    revert l l' H0. fix 3. destruct 1. constructor; auto.
-    constructor. now apply eval_evals_ind. now apply eval_evals_ind0.
+    revert args args' H0. fix aux 3. destruct 1. constructor; auto.
+    constructor. now apply eval_evals_ind. now apply aux.
+    revert l l' H H1. fix aux 4. destruct 2. contradiction. constructor.
+    now apply eval_evals_ind.
+    destruct l. inv H2; constructor.
+    now apply aux.
+    revert l l' H H1. fix aux 4. destruct 2. contradiction. constructor.
+    now apply eval_evals_ind. destruct l. inv H2; constructor. now apply aux.
   Defined.
 
   (** Characterization of values for this reduction relation:
@@ -165,7 +205,7 @@ Section Wcbv.
   | value_tEvar ev l : value (tEvar ev l)
   | value_tLam na t b : value (tLambda na t b)
   | value_tProd na t u : value (tProd na t u)
-  | value_tInd i k : value (tInd i k)
+  | value_tInd i k l : List.Forall value l -> value (mkApps (tInd i k) l)
   | value_tConstruct i k u l : List.Forall value l -> value (mkApps (tConstruct i k u) l).
 
   Lemma value_values_ind : forall P : term -> Prop,
@@ -173,30 +213,52 @@ Section Wcbv.
        (forall (ev : nat) (l : list term), P (tEvar ev l)) ->
        (forall (na : name) (t b : term), P (tLambda na t b)) ->
        (forall (na : name) (t u : term), P (tProd na t u)) ->
-       (forall (i : inductive) (k : universe_instance), P (tInd i k)) ->
+       (forall (i : inductive) (k : universe_instance) l, List.Forall value l -> List.Forall P l -> P (mkApps (tInd i k) l)) ->
        (forall (i : inductive) (k : nat) (u : universe_instance) (l : list term),
         List.Forall value l -> List.Forall P l -> P (mkApps (tConstruct i k u) l)) -> forall t : term, value t -> P t.
   Proof.
     intros P ??????.
-    fix 2. destruct 1. 1-5:clear value_values_ind; auto.
+    fix value_values_ind 2. destruct 1. 1-4:clear value_values_ind; auto.
+    apply H3. apply H5.
+    revert l H5. fix aux 2. destruct 1. constructor; auto.
+    constructor. now apply value_values_ind. now apply aux.
     apply H4. apply H5.
-    revert l H5. fix 2. destruct 1. constructor; auto.
-    constructor. now apply value_values_ind. now apply value_values_ind0.
+    revert l H5. fix aux 2. destruct 1. constructor; auto.
+    constructor. now apply value_values_ind. now apply aux.
   Defined.
 
   (** The codomain of evaluation is only values:
       It means no redex can remain at the head of an evaluated term. *)
 
+  Lemma Forall2_right {A B} (P : B -> Prop) (l : list A) (l' : list B) :
+    Forall2 (fun x y => P y) l l' -> List.Forall (fun x => P x) l'.
+  Proof.
+    induction 1; constructor; auto.
+  Qed.
+
+  Lemma Forall2_non_nil {A B} (P : A -> B -> Prop) (l : list A) (l' : list B) :
+    Forall2 P l l' -> l <> nil -> l' <> nil.
+  Proof.
+    induction 1; congruence.
+  Qed.
+
   Lemma eval_to_value e e' : eval e e' -> value e'.
   Proof.
     induction 1 using eval_evals_ind; simpl; auto using value.
-    constructor. clear H0 IHeval. induction H1; now constructor.
+    eapply (value_tInd i u []); try constructor.
+    pose proof (value_tInd i u l'). forward H3.
+    apply (Forall2_right _ _ _ H2).
+    rewrite mkApps_tApp in H3; auto. simpl; auto. eauto using Forall2_non_nil.
+    eapply (value_tConstruct i k u []); try constructor.
+    pose proof (value_tConstruct i k u l'). forward H3.
+    apply (Forall2_right _ _ _ H2).
+    rewrite mkApps_tApp in H3; auto. simpl; auto. eauto using Forall2_non_nil.
   Qed.
 
   (** Evaluation preserves closedness: *)
   Lemma eval_closed : forall n t u, closedn n t = true -> eval t u -> closedn n u = true.
   Proof.
-    induction 2 using eval_evals_ind; simpl in *; eauto. eapply IHeval2.
+    induction 2 using eval_evals_ind; simpl in *; eauto. eapply IHeval3.
     admit.
   Admitted. (* FIXME complete *)
 
