template-coq/theories/Erasure/Erase.v
@@ -1,0 +1,271 @@
+(* Distributed under the terms of the MIT license.   *)
+
+From Coq Require Import Bool String List Program BinPos Compare_dec Omega.
+From Template Require Import Template utils monad_utils Ast univ Induction LiftSubst UnivSubst Typing Checker Retyping MetaTheory WcbvEval.
+From Template Require AstUtils ErasedTerm.
+Require Import String.
+Local Open Scope string_scope.
+Set Asymmetric Patterns.
+Import MonadNotation.
+
+Definition is_prop_sort s :=
+  match Universe.level s with
+  | Some l => Level.is_prop l
+  | None => false
+  end.
+
+Module E := ErasedTerm.
+
+Section Erase.
+  Context `{F : Fuel}.
+  Context (Σ : global_context).
+
+  Definition is_box c := match c with
+                         | E.tBox => true
+                         | _ => false
+                         end.
+
+
+  Definition on_snd_map {A B C} (f : B -> C) (p : A * B) :=
+    (fst p, f (snd p)).
+
+  Section EraseMfix.
+    Context (erase : forall (Γ : context) (t : term), typing_result E.term).
+
+    Definition erase_mfix Γ (defs : mfixpoint term) :=
+      let Γ' := (fix_decls defs ++ Γ)%list in
+      monad_map (fun d => dtype' <- erase Γ d.(dtype);;
+                        dbody' <- erase Γ' d.(dbody);;
+                        ret ({| dname := d.(dname); rarg := d.(rarg);
+                                dtype := dtype'; dbody := dbody' |})) defs.
+  End EraseMfix.
+  
+  Fixpoint erase (Γ : context) (t : term) : typing_result E.term :=
+    s <- sort_of Σ Γ t;;
+    if is_prop_sort s then ret E.tBox
+    else match t with
+    | tRel i => ret (E.tRel i)
+    | tVar n => ret (E.tVar n)
+    | tMeta m => ret (E.tMeta m)
+    | tEvar m l =>
+      l' <- monad_map (erase Γ) l;;
+      ret (E.tEvar m l')
+    | tSort u => ret (E.tSort u)
+    | tConst kn u => ret (E.tConst kn u)
+    | tInd kn u => ret (E.tInd kn u)
+    | tConstruct kn k u => ret (E.tConstruct kn k u)
+    | tCast t k ty => erase Γ t
+                      (* ty' <- erase Γ ty ;; *)
+                      (* ret (tCast t' k ty') *)
+    | tProd na b t => b' <- erase Γ b;;
+                      t' <- erase (vass na b :: Γ) t;;
+                      ret (E.tProd na b' t')
+    | tLambda na b t =>
+      b' <- erase Γ b;;
+      t' <- erase (vass na b :: Γ) t;;
+      ret (E.tLambda na b' t')
+    | tLetIn na b t0 t1 =>
+      b' <- erase Γ b;;
+      t0' <- erase Γ t0;;
+      t1' <- erase (vdef na b t0 :: Γ) t1;;
+      ret (E.tLetIn na b' t0' t1')
+    | tApp f l =>
+      f' <- erase Γ f;;
+      l' <- monad_map (erase Γ) l;;
+      ret (E.tApp f' l') (* if is_dummy f' then ret dummy else *)
+    | tCase ip p c brs =>
+      c' <- erase Γ c;;
+      if is_box c' then
+        match brs with
+        | (_, x) :: _ => erase Γ x (* Singleton elimination *)
+        | nil =>
+          p' <- erase Γ p;;
+          ret (E.tCase ip p' c' nil) (* Falsity elimination *)
+        end
+      else
+        brs' <- monad_map (T:=typing_result) (fun x => x' <- erase Γ (snd x);; ret (fst x, x')) brs;;
+        p' <- erase Γ p;;
+        ret (E.tCase ip p' c' brs')
+    | tProj p c =>
+      c' <- erase Γ c;;
+      ret (E.tProj p c')
+    | tFix mfix n =>
+      mfix' <- erase_mfix erase Γ mfix;;
+      ret (E.tFix mfix' n)
+    | tCoFix mfix n =>
+      mfix' <- erase_mfix erase Γ mfix;;
+      ret (E.tCoFix mfix' n)
+     end.
+
+End Erase.
+
+(** * Erasure correctness
+    
+    The statement below expresses that any well-typed term's
+    extraction has the same operational semantics as its source, under
+    a few conditions:
+
+    - The terms has to be locally closed, otherwise evaluation could get 
+      stuck on free variables. Typing under an empty context ensures that.
+    - The global environment is axiom-free, for the same reason.
+    - The object is of inductive type, or more generally a function resulting 
+      ultimately in an inductive value when applied.
+
+   We use an observational equality relation to relate the two values, 
+   which is indifferent to the erased parts.
+ *)
+
+Fixpoint inductive_arity (t : term) :=
+  match t with
+  | tApp f _ | f =>
+    match f with
+    | tInd ind u => Some ind
+    | _ => None
+    end
+  end.
+
+(* Inductive inductive_arity : term -> Prop := *)
+(* | inductive_arity_concl ind u args : inductive_arity (mkApps (tInd ind u) args) *)
+(* | inductive_arity_arrow na b t : inductive_arity t -> inductive_arity (tProd na b t). *)
+
+Definition option_is_none {A} (o : option A) :=
+  match o with
+  | Some _ => false
+  | None => true
+  end.
+
+Definition is_axiom_decl g :=
+  match g with
+  | ConstantDecl kn cb => option_is_none cb.(cst_body)
+  | InductiveDecl kn ind => false
+  end.
+
+Definition axiom_free Σ :=
+  List.forallb (fun g => negb (is_axiom_decl g)) Σ.
+
+Definition computational_ind Σ ind :=
+  let 'mkInd mind n := ind in
+  let mib := lookup_env Σ mind in
+  match mib with
+  | Some (InductiveDecl kn decl) =>
+    match List.nth_error decl.(ind_bodies) n with
+    | Some body =>
+      match destArity [] body.(ind_type) with
+      | Some arity => negb (is_prop_sort (snd arity))
+      | None => false
+      end
+    | None => false
+    end
+  | _ => false
+  end.
+
+Require Import Bool.
+Coercion is_true : bool >-> Sortclass.
+
+Definition computational_type Σ T :=
+  exists ind, inductive_arity T = Some ind /\ computational_ind Σ ind.
+
+(** The precondition on the extraction theorem. *)
+
+Record extraction_pre (Σ : global_context) t T :=
+  { extr_typed : Σ ;;; [] |- t : T;
+    extr_env_axiom_free : axiom_free (fst Σ);
+    extr_computational_type : computational_type Σ T }.
+
+(** The observational equivalence relation between source and erased values. *)
+
+Definition destApp t :=
+  match t with
+  | tApp f args => (f, args)
+  | f => (f, [])
+  end.
+
+Inductive Question : Set  := 
+| Cnstr : Ast.inductive -> nat -> Question 
+| Abs : Question.
+
+Definition observe (q : Question) (v : E.term) : bool :=
+  match q with
+  | Cnstr i k =>
+    match v with
+    | E.tConstruct i' k' u =>
+      eq_ind i i' && eq_nat k k'
+    | _ => false
+    end
+  | Abs =>
+    match v with
+    | E.tLambda _ _ _ => true
+    | E.tFix _ _ => true
+    | _ => false
+    end
+  end.
+             
+
+(*
+Fixpoint obs_eq (Σ : global_context) (v v' : term) (T : term) (s : universe) : Prop :=
+  if is_prop_sort s then is_dummy v'
+  else
+    match T with
+    | tInd ind u =>
+      (* Canonical inductive value *)
+      let '(hd, args) := destApp v in
+      let '(hd', args') := destApp v' in
+      eq_term Σ hd hd' /\ obs_eq 
+      
+ | obs_eq_prf v T s : Σ ;;; [] |- v : T ->
+  Σ ;;; [] |- T : tSort s ->
+  is_prop_sort s ->
+  obs_eq Σ v dummy
+
+| obs_eq_cstr ind k u args args' T : Σ ;;; [] |- mkApps (tConstruct ind k u) args : T ->
+  computational_type Σ T ->
+  Forall2 (obs_eq Σ) args args' ->
+  obs_eq Σ (mkApps (tConstruct ind k u) args) (mkApps (tConstruct ind k u) args')
+
+| obs_eq_arrow na f f' T T' :
+    Σ ;;; [] |- f : tProd na T T' ->
+    (forall arg arg', obs_eq Σ arg arg' -> 
+    
+    obs_eq Σ f f'.                                     
+*)                      
+
+Record extraction_post (Σ : global_context) (t' v : term) :=
+  { extr_value : E.term;
+    extr_eval : EEval.eval Σ [] t' extr_value;
+    (* extr_equiv : obs_eq Σ v extr_value *) }.
+    
+
+
+(** The extraction correctness theorem we conjecture. *)
+
+Definition erasure_correctness :=
+  forall Σ t T, extraction_pre Σ t T ->
+    forall (f : Fuel) (t' : term),
+      erase Σ [] t = Checked t' ->
+      forall v, eval Σ [] t v ->
+      exists v', E.EEval Σ [] t' v'.
+      
+Conjecture erasure_correct : erasure_correctness.
+
+Quote Recursively Definition zero_syntax := 0.
+
+Definition erase_rec (t : global_declarations * term) : typing_result term :=
+  let '(Σ, t) := t in
+  erase (reconstruct_global_context Σ) [] t.
+
+(* A few tests *)
+
+Quote Recursively Definition true_syntax := I.
+Eval vm_compute in erase_rec true_syntax.
+
+Quote Recursively Definition exist_syntax := (exist _ 0 I : { x : nat | True }).
+Eval vm_compute in erase_rec exist_syntax.
+
+Quote Recursively Definition exist'_syntax := ((exist _ (S 0) (le_n (S 0))) : { x : nat | 0 < x }).
+Eval vm_compute in erase_rec exist'_syntax.
+
+Quote Recursively Definition fun_syntax := (fun (x : nat) (bla : x < 0) => x).
+Eval vm_compute in erase_rec fun_syntax. (* Not erasing bindings *)
+
+Quote Recursively Definition fun'_syntax := (fun (x : nat) (bla : x < 0) => bla).
+Eval vm_compute in erase_rec fun'_syntax. 
